src/Lean/Meta/Tactic/Cbv.lean
@@ -11,9 +11,9 @@ public import Lean.Meta.Tactic.Cbv.Main
 
 public section
 
--- namespace Lean
+namespace Lean
 
--- builtin_initialize registerTraceClass `Meta.Tactic.simp
+builtin_initialize registerTraceClass `Meta.Tactic.cbv
 -- builtin_initialize registerTraceClass `Meta.Tactic.simp.congr (inherited := true)
 -- builtin_initialize registerTraceClass `Meta.Tactic.simp.discharge (inherited := true)
 -- builtin_initialize registerTraceClass `Meta.Tactic.simp.rewrite (inherited := true)
@@ -22,7 +22,7 @@ public section
 -- builtin_initialize registerTraceClass `Meta.Tactic.simp.loopProtection (inherited := true)
 -- builtin_initialize registerTraceClass `Meta.Tactic.simp.numSteps
 -- builtin_initialize registerTraceClass `Meta.Tactic.simp.heads
--- builtin_initialize registerTraceClass `Debug.Meta.Tactic.simp
+builtin_initialize registerTraceClass `Debug.Meta.Tactic.cbv
 -- builtin_initialize registerTraceClass `Debug.Meta.Tactic.simp.congr (inherited := true)
 
--- end Lean
+end Lean
